\chapter{Equations}

\begin{definition}[Equation 1]\label{eq1}  Equation 1 is the law $x=x$.
\end{definition}

\begin{definition}[Equation 2]\label{eq2}  Equation 2 is the law $x=y$.
\end{definition}

\begin{definition}[Equation 3]\label{eq3}  Equation 3 is the law $x=x \circ x$.
\end{definition}

\begin{definition}[Equation 4]\label{eq4}  Equation 4 is the law $x=x \circ y$.
\end{definition}

\begin{definition}[Equation 5]\label{eq5}  Equation 5 is the law $x=y \circ x$.
\end{definition}

\begin{definition}[Equation 6]\label{eq6}  Equation 6 is the law $x=y \circ y$.
\end{definition}

\begin{definition}[Equation 7]\label{eq7}  Equation 7 is the law $x=y \circ z$.
\end{definition}

\begin{definition}[Equation 8]\label{eq8}  Equation 8 is the law $x=x \circ (x \circ x)$.
\end{definition}

\begin{definition}[Equation 42]\label{eq42}  Equation 42 is the law $x \circ y = x \circ z$.
\end{definition}

\begin{definition}[Equation 43]\label{eq43}  Equation 43 is the law $x \circ y = y \circ x$.
\end{definition}

\begin{definition}[Equation 46]\label{eq46}  Equation 46 is the law $x \circ y = z \circ w$.
\end{definition}

\begin{definition}[Equation 387]\label{eq387}  Equation 387 is the law $x \circ y = (y \circ y) \circ x$.
\end{definition}

\begin{definition}[Equation 4512]\label{eq4512}  Equation 4512 is the law $x \circ (y \circ z) = (x \circ y) \circ z$.
\end{definition}

\begin{definition}[Equation 4513]\label{eq4513}  Equation 4513 is the law $x \circ (y \circ z) = (x \circ y) \circ w$.
\end{definition}

\begin{definition}[Equation 4552]\label{eq4552}  Equation 4552 is the law $x \circ (y \circ z) = (x \circ w) \circ u$.
\end{definition}

\begin{definition}[Equation 4582]\label{eq4582}  Equation 4582 is the law $x \circ (y \circ z) = (w \circ u) \circ v$.
\end{definition}
